otbn_model/code/addc512_lemmas.dfy
@@ -1,7 +1,7 @@
 include "../spec/rsa_ops.dfy"
-include "../dafny_library/NonlinearArithmetic/Power.dfy"
-include "../dafny_library/NonlinearArithmetic/DivMod.dfy"
-include "../dafny_library/Sequences/Seq.dfy"
+include "../libraries/src/NonlinearArithmetic/Power.dfy"
+include "../libraries/src/NonlinearArithmetic/DivMod.dfy"
+include "../libraries/src/Collections/Sequences/Seq.dfy"
 
 module addc512_lemmas {
     import opened bv_ops
@@ -11,22 +11,16 @@ module addc512_lemmas {
     import opened Power
     import opened DivMod
     import NT = NativeTypes
-    import S = Seq
-    import refining_NatSeq
+    import opened Seq
+    import opened BASE_256_Seq
 
     lemma addc_256_op_lemma(
         x: uint256, y: uint256, z: uint256, c: uint1)
         requires (z, c) == uint256_addc(x, y, 0);
-        ensures seq_addc([x], [y]) == ([z], c);
+        ensures SeqAdd([x], [y]) == ([z], c);
     {
-        var (a, b) := refining_NatSeq.seq_add([x], [y]);
+        reveal SeqAdd();
         assert [] + [z] == [z];
-        calc {
-            seq_addc([x], [y]);
-            refining_NatSeq.seq_add([x], [y]);
-            (a, b);
-        }
-
     }
 
     lemma addc_512_op_lemma(
@@ -34,41 +28,34 @@ module addc512_lemmas {
         x1: uint256, y1: uint256, z1: uint256, c1: uint1)
         requires (z0, c0) == uint256_addc(x0, y0, 0);
         requires (z1, c1) == uint256_addc(x1, y1, c0);
-        ensures seq_addc([x0, x1], [y0, y1]) == ([z0, z1], c1);
+        ensures SeqAdd([x0, x1], [y0, y1]) == ([z0, z1], c1);
     {
+        reveal SeqAdd();
         addc_256_op_lemma(x0, y0, z0, c0);
         assert [z0] + [z1] == [z0, z1];
-
-        reveal refining_NatSeq.seq_add();
-        var (a, b) := refining_NatSeq.seq_add([x0, x1], [y0, y1]);
-        calc {
-            seq_addc([x0, x1], [y0, y1]);
-            refining_NatSeq.seq_add([x0, x1], [y0, y1]);
-            (a, b);
-        }
     }
 
     predicate seq_addc_512_is_safe(xs: seq<uint256>, ys: seq<uint256>)
         requires |xs| == |ys| == 2;
     {
-        to_nat(xs) + to_nat(ys) < pow_B256(2)
+        ToNat(xs) + ToNat(ys) < pow_B256(2)
     }
 
     lemma mont_word_mul_add_bound_lemma_0(
         xs: seq<uint256>, ys: seq<uint256>, a: uint256, b: uint256)
         requires |xs| == |ys| == 2;
-        requires to_nat(xs) == a * b;
-        requires S.last(ys) == 0;
+        requires ToNat(xs) == a * b;
+        requires Last(ys) == 0;
         ensures seq_addc_512_is_safe(xs, ys);
     {
-        var c := S.first(ys);
+        var c := First(ys);
         calc {
-            to_nat(xs) + to_nat(ys);
-            == { to_nat_lemma_1(ys); }
+            ToNat(xs) + ToNat(ys);
+            == { LemmaSeqLen2(ys); }
             a * b + c;
             < { single_digit_lemma_1(a, b, c, NT.BASE_256 - 1); }
             NT.BASE_256 * NT.BASE_256;
-            == { reveal power(); }
+            == { reveal Pow(); }
             pow_B256(2);
         }
     }
@@ -76,18 +63,18 @@ module addc512_lemmas {
     lemma mont_word_mul_add_bound_lemma_1(
         xs: seq<uint256>, ys: seq<uint256>, a: uint256, b: uint256, c: uint256)
         requires |xs| == |ys| == 2;
-        requires to_nat(xs) == a * b + c;
-        requires S.last(ys) == 0;
+        requires ToNat(xs) == a * b + c;
+        requires Last(ys) == 0;
         ensures seq_addc_512_is_safe(xs, ys);
     {
-        var d := S.first(ys);
+        var d := First(ys);
         calc {
-            to_nat(xs) + to_nat(ys);
-            == { to_nat_lemma_1(ys); }
+            ToNat(xs) + ToNat(ys);
+            == { LemmaSeqLen2(ys); }
             a * b + c + d;
             < { single_digit_lemma_2(a, b, c, d, NT.BASE_256 - 1); }
             NT.BASE_256 * NT.BASE_256;
-            == { reveal power(); }
+            == { reveal Pow(); }
             pow_B256(2);
         }
     }
@@ -95,18 +82,18 @@ module addc512_lemmas {
     lemma seq_addc_512_safe_nat_lemma(
         xs: seq<uint256>, ys: seq<uint256>, zs: seq<uint256>, cout: uint1)
         requires |xs| == 2 && |ys| == 2;
-        requires seq_addc(xs, ys) == (zs, cout);
+        requires SeqAdd(xs, ys) == (zs, cout);
         requires seq_addc_512_is_safe(xs, ys);
-        ensures to_nat(xs) + to_nat(ys) == to_nat(zs);
-        ensures to_nat(zs) < NT.BASE_512
+        ensures ToNat(xs) + ToNat(ys) == ToNat(zs);
+        ensures ToNat(zs) < NT.BASE_512
     {
         assert pow_B256(2) == NT.BASE_512 by {
-            reveal power();
+            reveal Pow();
         }
-        seq_addc_nat_lemma(xs, ys, zs, cout);
+        LemmaSeqAdd(xs, ys, zs, cout);
         if cout == 1 {
             assert false; // prove by contradiction
         }
-        assert to_nat(xs) + to_nat(ys) == to_nat(zs);
+        assert ToNat(xs) + ToNat(ys) == ToNat(zs);
     }
 }
